\documentclass[fleqn,12pt]{article}

\usepackage[margin=20mm]{geometry}
\usepackage[T2A]{fontenc}
\usepackage[utf8]{inputenc}
\usepackage[english,bulgarian]{babel}
\usepackage[document]{ragged2e}
\usepackage{amsthm}
\usepackage{amssymb}
\usepackage{mathtools}
\usepackage[unicode]{hyperref}

\hypersetup{
    colorlinks,
    linktoc=all,
    citecolor=black,
    filecolor=black,
    linkcolor=black,
    urlcolor=black
}

\newtheorem*{Th}{Теорема}
\newtheorem*{Lem}{Лема}
\newtheorem*{Def}{Дефиниция}
\newtheorem*{Claim}{Твърдение}
\newtheorem*{Corollary}{Следствие}

\renewcommand\qedsymbol{$\blacksquare$}

\title{Държавен СИ, юли 2021}
\date{13 юли 2021}

\begin{document}

\maketitle

\section{Задача 7}
Да се реши определеният интеграл.

\begin{gather*}
    \int_{-\pi/2}^{\pi/2} e^{|x|}(sinx + cosx) \; dx
\end{gather*}

\vspace{10pt}

\textbf{Решение}: 

Ясно е, че $e^{|x|} > 0$ за всяко реално $x$. Тогава имаме, че
\begin{gather*}
    e^{|x|} = 
    \begin{cases}
        e^x, x \geq 0 \\
        e^{-x}, x < 0
    \end{cases}
\end{gather*}

\begin{gather*} 
    \int_{-\pi/2}^{\pi/2} e^{|x|}(sinx + cosx) dx \\
    = \int_{-\pi/2}^{0} e^{-x}(sinx + cosx) \; dx + \int_{0}^{\pi/2} e^{x}(sinx + cosx) \; dx \\
    = I_1 + I_2
\end{gather*}

\begin{gather*}
    I_1 = \int_{-\pi/2}^{0} e^{-x}(sinx + cosx) dx \\
    = \int_{-\pi/2}^{0} e^{-x}sinx \; dx + \int_{-\pi/2}^{0} e^{-x}cosx \; dx \\
    = -\int_{-\pi/2}^{0} e^{-x} \; d(cosx) + \int_{-\pi/2}^{0} e^{-x}cosx \; dx \\
    = -e^{-x}cosx | ^{0}_{-\pi/2} + \int_{-\pi/2}^{0} cosx \; d(e^{-x}) + \int_{-\pi/2}^{0} e^{-x}cosx \; dx \\
    = -e^{0}cos(0) - \int_{-\pi/2}^{0} e^{-x}cosx \; dx + \int_{-\pi/2}^{0} e^{-x}cosx \; dx \\
    = - 1
\end{gather*}

\begin{gather*}
    I_2 = \int_{0}^{\pi/2} e^{x}(sinx + cosx) \; dx \\
    = \int_{0}^{\pi/2} e^{x}sinx \; dx + \int_{0}^{\pi/2} e^{x}cosx \; dx \\
    = \int_{0}^{\pi/2} e^{x}sinx \; dx + \int_{0}^{\pi/2} e^{x} \; d(sinx) \\
    = \int_{0}^{\pi/2} e^{x}sinx \; dx + e^{x}sinx | ^{\pi/2}_{0} - \int_{0}^{\pi/2} sinx \; d(e^{x}) \\
    = \int_{0}^{\pi/2} e^{x}sinx \; dx + e^{\pi/2}sin(\pi/2) - \int_{0}^{\pi/2} e^{x}sinx \; dx \\
    = e^{\pi/2}
\end{gather*}

\begin{gather*}
    \Longrightarrow  I_1 + I_2 = -1 + e^{\pi/2}
\end{gather*}

\end{document}
